gol_in_gol_circuitScript.sml
@@ -6,35 +6,7 @@ open gol_simLib gol_rulesTheory boolSyntax computeLib cv_transLib
 
 val _ = new_theory "gol_in_gol_circuit";
 
-Definition union_blist2_def:
-  union_blist2 _ NONE Nil ls = ls ∧
-  union_blist2 m NONE (Falses n ls1) ls = union_blist2 (m + n) NONE ls1 ls ∧
-  union_blist2 m NONE (Cell a ls1) ls = union_blist2 m (SOME a) ls1 ls ∧
-  union_blist2 m (SOME a) ls1 Nil = Nil ∧
-  union_blist2 m (SOME a) ls1 (Falses n ls) = (
-    if m < n then mk_Falses m (Cell a (union_blist2 0 NONE ls1 (Falses (n - (m + 1)) ls)))
-    else mk_Falses n (union_blist2 (m - n) (SOME a) ls1 ls)) ∧
-  union_blist2 m (SOME a) ls1 (Cell b ls) = (
-    if m = 0 then Cell (build_Or a b) (union_blist2 0 NONE ls1 ls)
-    else Cell b (union_blist2 (m - 1) (SOME a) ls1 ls))
-End
-
-Theorem union_blist_eq:
-  (∀m ls1 ls. union_blist m ls1 ls = union_blist2 m NONE ls1 ls) ∧
-  (∀m a ls1 ls. union_blist' m a ls1 ls = union_blist2 m (SOME a) ls1 ls)
-Proof
-  HO_MATCH_MP_TAC union_blist_ind
-  \\ simp [union_blist_def, union_blist2_def]
-QED
-
-(* val _ = cv_transLib.cv_trans_rec union_blist2_def (
-  WF_REL_TAC ‘measure (λ_,_,ls1,ls. cv$cv_size ls1 + cv$cv_size ls)’
-  \\ Cases \\ gvs [] \\ rw [] \\ gvs [])
-  (fn goal => (set_goal goal; PolyML.print goal; NO_TAC goal))
-) *)
-
-val _ = cv_transLib.cv_trans_rec union_blist2_def cheat
-val _ = cv_transLib.cv_trans union_blist_eq
+val _ = cv_transLib.cv_trans union_blist_def
 val _ = cv_transLib.cv_auto_trans build_mega_cell_def
 
 Theorem floodfill_result = floodfill diag params;
